src/Config.fsti
@@ -17,3 +17,8 @@ noextract inline_for_extraction
 val alg_null: v:nat{v = US.v metadata_max + 1}
 noextract inline_for_extraction
 val alg_null_sizet: v:US.t{US.v v = US.v metadata_max + 1}
+
+inline_for_extraction
+val enable_guard_pages: bool
+inline_for_extraction
+val guard_pages_interval: US.t
